thys/Untyped_Lambda_Calculus/LC_pair.thy
@@ -1,0 +1,1230 @@
+theory LC_pair
+  imports
+  "HOL-Library.FSet"
+  "Prelim.FixedCountableVars"
+  "Prelim.Swapping_vs_Permutation"
+  "Binders.General_Customization"
+  "Prelim.More_List"
+begin
+
+(* DATATYPE DECLARTION  *)
+
+declare [[mrbnf_internals]]
+binder_datatype 'a "term" =
+  Var 'a
+| App "'a term" "'a term"
+| Lam xy ::"'a \<times> 'a" t::"'a term" binds xy in t
+for
+  vvsubst: vvsubst
+  tvsubst: tvsubst 
+
+(****************************)
+(* DATATYPE-SPECIFIC CUSTOMIZATION  *)
+
+
+(* Monomorphising: *)
+instance var :: var_term_pre apply standard
+  using Field_natLeq infinite_iff_card_of_nat infinite_var
+  by (auto simp add: regularCard_var)
+
+instance var::cinf
+apply standard 
+  subgoal apply(rule exI[of _ "inv Variable"])
+  by (simp add: bij_Variable bij_is_inj)
+  subgoal using infinite_var . .
+
+type_synonym trm = "var term"
+
+(* Some lighter notations: *)
+abbreviation "VVr \<equiv> tvVVr_tvsubst"
+lemmas VVr_def = tvVVr_tvsubst_def
+abbreviation "isVVr \<equiv> tvisVVr_tvsubst"
+lemmas isVVr_def = tvisVVr_tvsubst_def
+abbreviation "IImsupp \<equiv> IImsupp_tvsubst"
+lemmas IImsupp_def = IImsupp_tvsubst_def
+abbreviation "SSupp \<equiv> SSupp_tvsubst"
+lemmas SSupp_def = SSupp_tvsubst_def
+abbreviation "FFVars \<equiv> FFVars_term"
+
+abbreviation "rrename \<equiv> rrename_term"
+(* *)
+
+lemma FFVars_tvsubst[simp]:
+  assumes "|SSupp (\<sigma> :: var \<Rightarrow> trm)| <o |UNIV :: var set|"
+  shows "FFVars (tvsubst \<sigma> t) = (\<Union> {FFVars (\<sigma> x) | x . x \<in> FFVars t})"
+  apply (binder_induction t avoiding: "IImsupp \<sigma>" rule: term.strong_induct)
+     apply (auto simp: IImsupp_def assms intro!: Un_bound UN_bound term.card_of_FFVars_bounds)
+  using term.FVars_VVr apply (fastforce simp add: SSupp_def)
+  using term.FVars_VVr apply (auto simp add: SSupp_def)
+  by (smt (verit) singletonD term.FVars_VVr)
+
+lemma fsupp_le[simp]: 
+"fsupp (\<sigma>::var\<Rightarrow>var) \<Longrightarrow> |supp \<sigma>| <o |UNIV::var set|" 
+by (simp add: finite_card_var fsupp_def supp_def)
+
+(* Enabling some simplification rules: *)
+lemmas term.tvsubst_VVr[simp] term.FVars_VVr[simp]
+term.rrename_ids[simp] term.rrename_cong_ids[simp]
+term.FFVars_rrenames[simp]
+
+lemma singl_bound: "|{a}| <o |UNIV::var set|"
+  by (rule finite_ordLess_infinite2[OF finite_singleton cinfinite_imp_infinite[OF term_pre.UNIV_cinfinite]])
+
+lemma ls_UNIV_iff_finite: "|A| <o |UNIV::var set| \<longleftrightarrow> finite A"
+using finite_iff_le_card_var by blast
+
+lemma supp_id_update_le[simp,intro]:
+"|supp (id(x := y))| <o |UNIV::var set|"
+by (metis finite.emptyI finite.insertI finite_card_var imsupp_id_fun_upd imsupp_supp_bound infinite_var)
+
+lemma IImsupp_VVr_empty[simp]: "IImsupp VVr = {}"
+  unfolding IImsupp_def
+  term.SSupp_VVr_empty UN_empty Un_empty_left
+  apply (rule refl)
+  done
+
+(* VVr is here the Var constructor: *)
+lemma VVr_eq_Var[simp]: "VVr = Var"
+  unfolding VVr_def Var_def comp_def
+  tv\<eta>_term_tvsubst_def
+  by (rule refl)
+
+(* *)
+(* Properties of term-for-variable substitution *)
+
+lemma tvsubst_VVr_func[simp]: "tvsubst VVr t = t"
+  apply (rule term.TT_plain_co_induct)
+  subgoal for x
+    apply (rule case_split[of "isVVr (term_ctor x)"])
+     apply (unfold isVVr_def)[1]
+     apply (erule exE)
+    subgoal premises prems for a
+      unfolding prems
+      apply (rule term.tvsubst_VVr)
+      apply (rule term.SSupp_VVr_bound)
+        done
+      apply (rule trans)
+       apply (rule term.tvsubst_cctor_not_isVVr)
+          apply (rule term.SSupp_VVr_bound)
+      unfolding IImsupp_VVr_empty
+         apply (rule Int_empty_right)
+      unfolding noclash_term_def Int_Un_distrib Un_empty
+        apply (rule conjI)
+         apply (rule iffD2[OF disjoint_iff], rule allI, rule impI, assumption)
+        apply (rule iffD2[OF disjoint_iff], rule allI, rule impI)
+      unfolding UN_iff Set.bex_simps
+        apply (rule ballI)
+        apply assumption+
+      apply (rule arg_cong[of _ _ term_ctor])
+      apply (rule trans)
+      apply (rule term_pre.map_cong)
+                 apply (rule supp_id_bound bij_id)+
+           apply (assumption | rule refl)+
+      unfolding id_def[symmetric] term_pre.map_id
+      apply (rule refl)
+      done
+    done
+
+proposition rrename_simps[simp]:
+  assumes "bij (f::var \<Rightarrow> var)" "|supp f| <o |UNIV::var set|"
+  shows "rrename f (Var a) = Var (f a)"
+    "rrename f (App e1 e2) = App (rrename f e1) (rrename f e2)"
+    "rrename f (Lam x e) = Lam (f x) (rrename f e)"
+  unfolding Var_def App_def Lam_def term.rrename_cctors[OF assms] map_term_pre_def comp_def
+    Abs_term_pre_inverse[OF UNIV_I] map_sum_def sum.case map_prod_def prod.case id_def
+    apply (rule refl)+
+  done
+
+lemma rrename_cong:
+assumes "bij f" "|supp f| <o |UNIV::var set|" "bij g" "|supp g| <o |UNIV::var set|"
+"(\<And>z. (z::var) \<in> FFVars P \<Longrightarrow> f z = g z)"
+shows "rrename f P = rrename g P"
+using assms(5) apply(binder_induction P avoiding: "supp f" "supp g" rule: term.strong_induct)
+using assms apply auto by (metis not_in_supp_alt)+
+
+lemma tvsubst_cong:
+assumes f: "|SSupp f| <o |UNIV::var set|" and g: "|SSupp g| <o |UNIV::var set|"
+and eq: "(\<And>z. (z::var) \<in> FFVars P \<Longrightarrow> f z = g z)"
+shows "tvsubst f P = tvsubst g P"
+proof-
+  have fg: "|IImsupp f| <o |UNIV::var set|" "|IImsupp g| <o |UNIV::var set|" 
+    using f g  
+    by (simp_all add: IImsupp_def term.card_of_FFVars_bounds 
+       term_prevar_term_prevar_term_prevar_prodIDterm_prevar_prodIDsum_class.UN_bound 
+       term_prevar_term_prevar_term_prevar_prodIDterm_prevar_prodIDsum_class.Un_bound) 
+  have 0: "|IImsupp f \<union> IImsupp g| <o |UNIV::var set|" 
+    using fg var_term_pre_class.Un_bound by blast
+  show ?thesis using 0 eq apply(binder_induction P avoiding: "IImsupp f" "IImsupp g" rule: term.strong_induct)
+    subgoal using fg by auto
+    subgoal using fg by simp  
+    subgoal using f g by simp
+    subgoal using f g by simp
+    subgoal using f g fg apply simp unfolding IImsupp_def SSupp_def 
+    by auto metis .
+qed
+
+proposition App_inject[simp]: "(App a b = App c d) = (a = c \<and> b = d)"
+proof
+  assume "App a b = App c d"
+  then show "a = c \<and> b = d"
+    unfolding App_def fun_eq_iff term.TT_injects0
+      map_term_pre_def comp_def Abs_term_pre_inverse[OF UNIV_I] map_sum_def sum.case prod.map_id
+      Abs_term_pre_inject[OF UNIV_I UNIV_I]
+    by blast
+qed simp
+
+proposition Var_inject[simp]: "(Var a = Var b) = (a = b)"
+  apply (rule iffI[rotated])
+   apply (rule arg_cong[of _ _ Var])
+  apply assumption
+  unfolding Var_def term.TT_injects0 map_term_pre_def comp_def map_sum_def sum.case Abs_term_pre_inverse[OF UNIV_I]
+  id_def Abs_term_pre_inject[OF UNIV_I UNIV_I] sum.inject
+  apply (erule exE conjE)+
+  apply assumption
+  done
+
+lemma Lam_inject: "(Lam x e = Lam x' e') = (\<exists>f. bij f \<and> |supp (f::var \<Rightarrow> var)| <o |UNIV::var set|
+  \<and> id_on (FFVars_term (Lam x e)) f \<and> f x = x' \<and> rrename f e = e')"
+  unfolding term.set
+  unfolding Lam_def term.TT_injects0 map_term_pre_def comp_def Abs_term_pre_inverse[OF UNIV_I]
+    map_sum_def sum.case map_prod_def prod.case id_def Abs_term_pre_inject[OF UNIV_I UNIV_I] sum.inject prod.inject
+    set3_term_pre_def sum_set_simps Union_empty Un_empty_left prod_set_simps cSup_singleton set2_term_pre_def
+    Un_empty_right UN_single
+  apply (rule refl)
+  done
+
+lemma Lam_same_inject[simp]: "Lam (x::var) e = Lam x e' \<longleftrightarrow> e = e'"
+unfolding Lam_inject apply safe
+apply(rule term.rrename_cong_ids[symmetric]) 
+unfolding id_on_def by auto
+
+lemma bij_map_term_pre: "bij f \<Longrightarrow> |supp (f::var \<Rightarrow> var)| <o |UNIV::var set| \<Longrightarrow> bij (map_term_pre (id::var \<Rightarrow>var) f (rrename f) id)"
+  apply (rule iffD2[OF bij_iff])
+    apply (rule exI[of _ "map_term_pre id (inv f) (rrename (inv f)) id"])
+  apply (frule bij_imp_bij_inv)
+  apply (frule supp_inv_bound)
+   apply assumption
+  apply (rule conjI)
+   apply (rule trans)
+    apply (rule term_pre.map_comp0[symmetric])
+         apply (assumption | rule supp_id_bound)+
+  unfolding id_o inv_o_simp1 term.rrename_comp0s term.rrename_id0s
+  apply (rule term_pre.map_id0)
+  apply (rule trans)
+   apply (rule term_pre.map_comp0[symmetric])
+        apply (assumption | rule supp_id_bound)+
+  unfolding id_o inv_o_simp2 term.rrename_comp0s term.rrename_id0s
+  apply (rule term_pre.map_id0)
+  done
+
+lemma map_term_pre_inv_simp: "bij f \<Longrightarrow> |supp (f::var \<Rightarrow> var)| <o |UNIV::var set| \<Longrightarrow> inv (map_term_pre (id::_::var_term_pre \<Rightarrow> _) f (rrename f) id) = map_term_pre id (inv f) (rrename (inv f)) id"
+  apply (frule bij_imp_bij_inv)
+  apply (frule supp_inv_bound)
+  apply assumption
+  apply (rule inv_unique_comp)
+   apply (rule trans)
+    apply (rule term_pre.map_comp0[symmetric])
+         apply (assumption | rule supp_id_bound)+
+   defer
+  apply (rule trans)
+    apply (rule term_pre.map_comp0[symmetric])
+         apply (assumption | rule supp_id_bound)+
+  unfolding id_o inv_o_simp1 inv_o_simp2 term.rrename_comp0s term.rrename_id0s term_pre.map_id0
+   apply (rule refl)+
+  done
+
+lemma Lam_set3: "term_ctor v = Lam (x::var) e \<Longrightarrow> \<exists>x' e'. term_ctor v = Lam x' e' \<and> x' \<in> set2_term_pre v \<and> e' \<in> set3_term_pre v"
+  unfolding Lam_def term.TT_injects0
+  apply (erule exE)
+  apply (erule conjE)+
+  subgoal for f
+apply (drule iffD2[OF bij_imp_inv', rotated, of "map_term_pre id f (rrename f) id"])
+     apply (rule bij_map_term_pre)
+      apply assumption+
+    apply (rule exI)
+    apply (rule exI)
+    apply (rule conjI)
+     apply (rule exI[of _ "id"])
+     apply (rule conjI bij_id supp_id_bound id_on_id)+
+    apply (drule sym)
+    unfolding term.rrename_id0s term_pre.map_id map_term_pre_inv_simp
+    unfolding map_term_pre_def comp_def Abs_term_pre_inverse[OF UNIV_I] map_sum_def sum.case
+      map_prod_def prod.case id_def
+    apply assumption
+    apply (raw_tactic \<open>hyp_subst_tac @{context} 1\<close>)
+unfolding set2_term_pre_def set3_term_pre_def comp_def Abs_term_pre_inverse[OF UNIV_I] sum_set_simps
+    map_sum_def sum.case Union_empty Un_empty_left map_prod_def prod.case prod_set_simps
+      ccpo_Sup_singleton Un_empty_right id_on_def image_single[symmetric]
+  unfolding term.FFVars_rrenames[OF bij_imp_bij_inv supp_inv_bound]
+  unfolding image_single image_set_diff[OF bij_is_inj[OF bij_imp_bij_inv], symmetric]
+    image_in_bij_eq[OF bij_imp_bij_inv] inv_inv_eq image_in_bij_eq[OF term.rrename_bijs[OF bij_imp_bij_inv supp_inv_bound]]
+  term.rrename_inv_simps[OF bij_imp_bij_inv supp_inv_bound] inv_simp2
+  unfolding term.rrename_comps[OF bij_imp_bij_inv supp_inv_bound] inv_o_simp2 term.rrename_ids
+  apply (rule conjI bij_imp_bij_inv supp_inv_bound singletonI | assumption)+
+  done
+  done
+
+lemma Lam_avoid: "|A::var set| <o |UNIV::var set| \<Longrightarrow> \<exists>x' e'. Lam x e = Lam x' e' \<and> x' \<notin> A"
+  apply (drule term.TT_fresh_nchotomys[of _ "Lam x e"])
+  apply (erule exE)
+  apply (erule conjE)
+   apply (drule sym)
+  apply (frule Lam_set3)
+  apply (erule exE conjE)+
+  apply (rule exI)+
+  apply (rule conjI)
+   apply (rule trans)
+    apply (rule sym)
+    apply assumption
+  apply (rotate_tac 2)
+   apply assumption
+  apply (drule iffD1[OF disjoint_iff])
+  apply (erule allE)
+  apply (erule impE)
+   apply assumption
+  apply assumption
+  done
+
+lemma Lam_rrename:
+"bij (\<sigma>::var\<Rightarrow>var) \<Longrightarrow> |supp \<sigma>| <o |UNIV:: var set| \<Longrightarrow>
+ (\<And>a'. a' \<in>FFVars_term e - {a::var} \<Longrightarrow> \<sigma> a' = a') \<Longrightarrow> Lam a e = Lam (\<sigma> a) (rrename \<sigma> e)"
+by (metis rrename_simps(3) term.rrename_cong_ids term.set(3))
+
+
+(* Bound properties (needed as auxiliaries): *)
+
+lemma SSupp_upd_bound:
+  fixes f::"var \<Rightarrow> trm"
+  shows "|SSupp (f (a:=t))| <o |UNIV::var set| \<longleftrightarrow> |SSupp f| <o |UNIV::var set|"
+  unfolding SSupp_def
+  by (auto simp only: fun_upd_apply singl_bound ordLeq_refl fset_simps split: if_splits
+      elim!: ordLeq_ordLess_trans[OF card_of_mono1 ordLess_ordLeq_trans[OF term_pre.Un_bound], rotated, of _ "{a}"]
+      intro: card_of_mono1)
+
+corollary SSupp_upd_VVr_bound[simp,intro!]: "|SSupp (VVr(a:=(t::trm)))| <o |UNIV::var set|"
+  apply (rule iffD2[OF SSupp_upd_bound])
+  apply (rule term.SSupp_VVr_bound)
+  done
+
+lemma SSupp_upd_Var_bound[simp,intro!]: "|SSupp (Var(a:=(t::trm)))| <o |UNIV::var set|"
+using SSupp_upd_VVr_bound by auto
+
+lemma supp_swap_bound[simp,intro!]: "|supp (id(x::var := xx, xx := x))| <o |UNIV:: var set|"
+by (simp add: cinfinite_imp_infinite supp_swap_bound term.UNIV_cinfinite)
+
+lemma SSupp_IImsupp_bound: "|SSupp \<sigma>| <o |UNIV:: var set| \<Longrightarrow> |IImsupp \<sigma>| <o |UNIV:: var set|"
+unfolding IImsupp_def
+by (simp add: var_ID_class.Un_bound term.set_bd_UNIV var_term_pre_class.UN_bound)
+
+(* *)
+
+lemma IImsupp_tvsubst_su:
+assumes s[simp]: "|SSupp \<sigma>| <o  |UNIV:: var set|"
+shows "IImsupp (tvsubst (\<sigma>::var\<Rightarrow>trm) o \<tau>) \<subseteq> IImsupp \<sigma> \<union> IImsupp \<tau>"
+unfolding IImsupp_def SSupp_def apply auto
+by (metis s singletonD term.set(1) term.subst(1))
+
+lemma IImsupp_tvsubst_su':
+assumes s[simp]: "|SSupp \<sigma>| <o  |UNIV:: var set|"
+shows "IImsupp (\<lambda>a. tvsubst (\<sigma>::var\<Rightarrow>trm) (\<tau> a)) \<subseteq> IImsupp \<sigma> \<union> IImsupp \<tau>"
+using IImsupp_tvsubst_su[OF assms] unfolding o_def .
+
+lemma IImsupp_tvsubst_bound:
+assumes s: "|SSupp \<sigma>| <o |UNIV:: var set|" "|SSupp \<tau>| <o |UNIV:: var set|"
+shows "|IImsupp (tvsubst (\<sigma>::var\<Rightarrow>trm) o \<tau>)| <o |UNIV:: var set|"
+using IImsupp_tvsubst_su[OF s(1)] s
+by (meson Un_bound SSupp_IImsupp_bound card_of_subset_bound)
+
+lemma SSupp_tvsubst_bound:
+assumes s: "|SSupp \<sigma>| <o |UNIV:: var set|" "|SSupp \<tau>| <o |UNIV:: var set|"
+shows "|SSupp (tvsubst (\<sigma>::var\<Rightarrow>trm) o \<tau>)| <o |UNIV:: var set|"
+using IImsupp_tvsubst_bound[OF assms]
+by (metis IImsupp_def card_of_subset_bound sup_ge1)
+
+lemma SSupp_tvsubst_bound':
+assumes s: "|SSupp \<sigma>| <o |UNIV:: var set|" "|SSupp \<tau>| <o |UNIV:: var set|"
+shows "|SSupp (\<lambda>a. tvsubst (\<sigma>::var\<Rightarrow>trm) (\<tau> a))| <o |UNIV:: var set|"
+using SSupp_tvsubst_bound[OF assms] unfolding o_def .
+
+(* *)
+
+lemma IImsupp_Var: "IImsupp (Var(x := e)) \<subseteq> FFVars e \<union> {x}"
+unfolding LC.IImsupp_def LC.SSupp_def by auto
+
+lemma IImsupp_Var': "y \<noteq> x \<and> y \<notin> FFVars e \<Longrightarrow> y \<notin> IImsupp (Var(x := e))"
+using IImsupp_Var by auto 
+
+lemma IImsupp_rrename_su:
+assumes s[simp]: "bij (\<sigma>::var\<Rightarrow>var)" "|supp \<sigma>| <o  |UNIV:: var set|"
+shows "IImsupp (rrename (\<sigma>::var\<Rightarrow>var) o \<tau>) \<subseteq> imsupp \<sigma> \<union> IImsupp \<tau>"
+unfolding IImsupp_def imsupp_def supp_def SSupp_def by force
+
+lemma IImsupp_rrename_su':
+assumes s[simp]: "bij (\<sigma>::var\<Rightarrow>var)" "|supp \<sigma>| <o  |UNIV:: var set|"
+shows "IImsupp (\<lambda>a. rrename (\<sigma>::var\<Rightarrow>var) (\<tau> a)) \<subseteq> imsupp \<sigma> \<union> IImsupp \<tau>"
+using IImsupp_rrename_su[OF assms] unfolding o_def .
+
+lemma IImsupp_rrename_bound:
+assumes s: "bij (\<sigma>::var\<Rightarrow>var)" "|supp \<sigma>| <o  |UNIV:: var set|" "|SSupp \<tau>| <o |UNIV:: var set|"
+shows "|IImsupp (rrename (\<sigma>::var\<Rightarrow>var) o \<tau>)| <o |UNIV:: var set|"
+using IImsupp_rrename_su[OF s(1,2)] s
+by (metis SSupp_IImsupp_bound finite_Un finite_iff_le_card_var finite_subset imsupp_supp_bound infinite_var)
+
+lemma SSupp_rrename_bound:
+assumes s: "bij (\<sigma>::var\<Rightarrow>var)" "|supp \<sigma>| <o  |UNIV:: var set|" "|SSupp \<tau>| <o |UNIV:: var set|"
+shows "|SSupp (rrename (\<sigma>::var\<Rightarrow>var) o \<tau>)| <o |UNIV:: var set|"
+using IImsupp_rrename_bound[OF assms]
+by (metis IImsupp_def card_of_subset_bound sup_ge1)
+
+lemma SSupp_rrename_bound':
+assumes s: "bij (\<sigma>::var\<Rightarrow>var)" "|supp \<sigma>| <o  |UNIV:: var set|" "|SSupp \<tau>| <o |UNIV:: var set|"
+shows "|SSupp (\<lambda>a. rrename (\<sigma>::var\<Rightarrow>var) (\<tau> a))| <o |UNIV:: var set|"
+using SSupp_rrename_bound[OF assms] unfolding o_def .
+
+(* *)
+lemma SSupp_update_rrename_bound:
+"|SSupp (Var(\<sigma> (x::var) := rrename \<sigma> e))| <o |UNIV::var set|"
+using SSupp_upd_Var_bound .
+
+lemma IImsupp_rrename_update_su:
+assumes s[simp]: "bij (\<sigma>::var\<Rightarrow>var)" "|supp \<sigma>| <o |UNIV::var set|"
+shows "IImsupp (rrename \<sigma> \<circ> Var(x := e)) \<subseteq>
+       imsupp \<sigma> \<union> {x} \<union> FFVars_term e"
+unfolding IImsupp_def SSupp_def imsupp_def supp_def by (auto split: if_splits)
+
+lemma IImsupp_rrename_update_bound:
+assumes s[simp]: "bij (\<sigma>::var\<Rightarrow>var)" "|supp \<sigma>| <o |UNIV::var set|"
+shows "|IImsupp (rrename \<sigma> \<circ> Var(x := e))| <o |UNIV::var set|"
+using IImsupp_rrename_update_su[OF assms]
+by (meson Un_bound card_of_subset_bound imsupp_supp_bound infinite_var s(2) singl_bound term.set_bd_UNIV)
+
+lemma SSupp_rrename_update_bound:
+assumes s[simp]: "bij (\<sigma>::var\<Rightarrow>var)" "|supp \<sigma>| <o |UNIV::var set|"
+shows "|SSupp (rrename \<sigma> \<circ> Var(x := e))| <o |UNIV::var set|"
+using IImsupp_rrename_update_bound[OF assms]
+  by (metis (mono_tags) IImsupp_def finite_Un finite_iff_le_card_var)
+
+(* Action of swapping (a particular renaming) on variables *)
+
+lemma rrename_swap_Var1[simp]: "rrename (id(x := xx, xx := x)) (Var (x::var)) = Var xx"
+apply(subst rrename_simps(1)) by auto
+lemma rrename_swap_Var2[simp]: "rrename (id(x := xx, xx := x)) (Var (xx::var)) = Var x"
+apply(subst rrename_simps(1)) by auto
+lemma rrename_swap_Var3[simp]: "z \<notin> {x,xx} \<Longrightarrow> rrename (id(x := xx, xx := x)) (Var (z::var)) = Var z"
+apply(subst rrename_simps(1)) by auto
+lemma rrename_swap_Var[simp]: "rrename (id(x := xx, xx := x)) (Var (z::var)) =
+ Var (if z = x then xx else if z = xx then x else z)"
+apply(subst rrename_simps(1)) by auto
+
+(* Compositionality properties of renaming and term-for-variable substitution *)
+
+lemma tvsubst_comp:
+assumes s[simp]: "|SSupp \<sigma>| <o |UNIV:: var set|" "|SSupp \<tau>| <o |UNIV:: var set|"
+shows "tvsubst (\<sigma>::var\<Rightarrow>trm) (tvsubst \<tau> e) = tvsubst (tvsubst \<sigma> \<circ> \<tau>) e"
+proof-
+  note SSupp_tvsubst_bound'[OF s, simp]
+  show ?thesis
+  apply(induct e rule: term.fresh_induct[where A = "IImsupp \<sigma> \<union> IImsupp \<tau>"])
+    subgoal using Un_bound[OF s]
+      using var_ID_class.Un_bound SSupp_IImsupp_bound s(1) s(2) by blast
+    subgoal by simp
+    subgoal by simp
+    subgoal for x t apply(subgoal_tac "x \<notin> IImsupp (\<lambda>a. tvsubst \<sigma> (\<tau> a))")
+      subgoal by simp
+      subgoal using IImsupp_tvsubst_su'[OF s(1)] by blast . .
+qed
+
+lemma rrename_tvsubst_comp:
+assumes b[simp]: "bij (\<sigma>::var\<Rightarrow>var)" and s[simp]: "|supp \<sigma>| <o |UNIV:: var set|" "|SSupp \<tau>| <o |UNIV:: var set|"
+shows "rrename \<sigma> (tvsubst \<tau> e) = tvsubst (rrename \<sigma> \<circ> \<tau>) e"
+proof-
+  note SSupp_rrename_bound'[OF b s, simp]
+  show ?thesis
+  apply(induct e rule: term.fresh_induct[where A = "IImsupp \<tau> \<union> imsupp \<sigma>"])
+    subgoal using s(1) s(2) Un_bound SSupp_IImsupp_bound imsupp_supp_bound infinite_var by blast
+    subgoal by simp
+    subgoal by simp
+    subgoal for x t apply simp apply(subgoal_tac "x \<notin> IImsupp (\<lambda>a. rrename  \<sigma> (\<tau> a))")
+      subgoal unfolding imsupp_def supp_def by simp
+      subgoal using IImsupp_rrename_su' b s(1) by blast . .
+qed
+
+
+(* Unary (term-for-var) substitution versus renaming: *)
+
+lemma supp_SSupp_Var_le[simp]: "SSupp (Var \<circ> \<sigma>) = supp \<sigma>" 
+unfolding supp_def SSupp_def by simp
+
+lemma rrename_eq_tvsubst_Var: 
+assumes "bij (\<sigma>::var\<Rightarrow>var)" "|supp \<sigma>| <o |UNIV::var set|" 
+shows "rrename \<sigma> = tvsubst (Var o \<sigma>)"
+proof
+  fix t
+  show "rrename \<sigma> t = tvsubst (Var o \<sigma>) t"
+  proof (binder_induction t avoiding: "IImsupp (Var \<circ> \<sigma>)" rule: term.strong_induct)
+    case Bound
+    then show ?case using assms SSupp_IImsupp_bound by (metis supp_SSupp_Var_le)
+  next
+    case (Lam x1 x2)
+    then show ?case by (simp add: assms IImsupp_def disjoint_iff not_in_supp_alt)
+  qed (auto simp: assms)
+qed
+     
+lemma rrename_eq_tvsubst_Var': 
+"bij (\<sigma>::var\<Rightarrow>var) \<Longrightarrow> |supp \<sigma>| <o |UNIV::var set| \<Longrightarrow> rrename \<sigma> e = tvsubst (Var o \<sigma>) e"
+using rrename_eq_tvsubst_Var by auto
+
+(* Equivariance of unary substitution: *)
+
+lemma tvsubst_rrename_comp[simp]:
+assumes s[simp]: "bij (\<sigma>::var\<Rightarrow>var)" "|supp \<sigma>| <o |UNIV::var set|"
+shows "tvsubst (rrename \<sigma> \<circ> Var(x := e2)) e1 = tvsubst (Var(\<sigma> x := rrename \<sigma> e2)) (rrename \<sigma> e1)"
+proof-
+  note SSupp_rrename_update_bound[OF assms, unfolded comp_def, simplified, simp]
+  note SSupp_update_rrename_bound[unfolded fun_upd_def, simplified, simp]
+  show ?thesis
+  apply(induct e1 rule: term.fresh_induct[where A = "{x} \<union> FFVars_term e2 \<union> imsupp \<sigma>"])
+    subgoal by (meson Un_bound imsupp_supp_bound infinite_var s(2) singl_bound term.set_bd_UNIV)
+    subgoal by auto
+    subgoal by simp
+    subgoal for y t apply simp apply(subgoal_tac
+      "y \<notin> IImsupp ((\<lambda>a. rrename \<sigma> (if a = x then e2 else Var a))) \<and>
+      \<sigma> y \<notin> IImsupp (\<lambda>a. if a = \<sigma> x then rrename \<sigma> e2 else Var a)")
+      subgoal unfolding imsupp_def supp_def by simp
+      subgoal unfolding IImsupp_def imsupp_def SSupp_def supp_def by auto . .
+qed
+
+(* Unary substitution versus swapping: *)
+lemma tvsubst_refresh:
+assumes xx: "xx \<notin> FFVars_term e1 - {x}"
+shows "tvsubst (Var((x::var) := e2)) e1 = tvsubst (Var(xx := e2)) (rrename (id(x := xx, xx := x)) e1)"
+proof-
+  show ?thesis using xx
+  apply(induct e1 rule: term.fresh_induct[where A = "{x,xx} \<union> FFVars_term e2"])
+    subgoal by (metis insert_is_Un term.set(1) term.set(2) term.set_bd_UNIV)
+    subgoal by simp
+    subgoal by auto
+    subgoal for y t apply simp apply(subgoal_tac
+      "y \<notin> IImsupp (Var(x := e2)) \<and> y \<notin> IImsupp (Var(xx := e2))")
+      subgoal unfolding imsupp_def supp_def by auto
+      subgoal unfolding IImsupp_def imsupp_def SSupp_def supp_def by auto . .
+qed
+
+(*   *)
+
+(* *)
+
+(* Swapping and unary substitution, as abbreviations: *)
+abbreviation "swap t (x::var) y \<equiv> rrename (id(x:=y,y:=x)) t"
+abbreviation "usub t (y::var) x \<equiv> vvsubst (id(x:=y)) t"
+
+(* *)
+
+lemma usub_swap_disj:
+assumes "{u,v} \<inter> {x,y} = {}"
+shows "usub (swap t u v) x y = swap (usub t x y) u v"
+proof-
+  note term_vvsubst_rrename[simp del]
+  show ?thesis using assms
+  apply(subst term_vvsubst_rrename[symmetric]) apply auto
+  apply(subst term.map_comp) apply auto
+  apply(subst term_vvsubst_rrename[symmetric]) apply auto
+  apply(subst term.map_comp) apply auto
+  apply(rule term.map_cong0)
+    using term_pre.supp_comp_bound by auto
+qed
+
+lemma rrename_o_swap:
+"rrename (id(y::var := yy, yy := y) o id(x := xx, xx := x)) t =
+ swap (swap t x xx) y yy"
+apply(subst term.rrename_comps[symmetric])
+by auto
+
+(* *)
+
+lemma swap_simps[simp]: "swap (Var z) (y::var) x = Var (sw z y x)"
+"swap (App t s) (y::var) x = App(swap t y x) (swap s y x)"
+"swap (Lam v t) (y::var) x = Lam (sw v y x) (swap t y x)"
+by (auto simp: sw_def)
+
+lemma FFVars_swap[simp]: "FFVars (swap t y x) =
+ (\<lambda>u. sw u x y) ` (FFVars t)"
+apply(subst term.FFVars_rrenames) by (auto simp: sw_def)
+
+lemma FFVars_swap'[simp]: "{x::var,y} \<inter> FFVars t = {} \<Longrightarrow> swap t x y = t"
+apply(rule term.rrename_cong_ids) by auto
+
+(* *)
+
+lemma Lam_inject_swap: "Lam v t = Lam v' t' \<longleftrightarrow>
+  (v' \<notin> FFVars t \<or> v' = v) \<and> swap t v' v = t'"
+unfolding Lam_inject apply(rule iffI)
+  subgoal unfolding id_on_def apply auto
+  apply(rule rrename_cong) by auto
+  subgoal apply clarsimp
+  apply(rule exI[of _ "id(v':=v,v:=v')"]) unfolding id_on_def by auto .
+
+lemma Lam_inject_swap': "Lam v t = Lam v' t' \<longleftrightarrow>
+  (\<exists>z. (z \<notin> FFVars t \<or> z = v) \<and> (z \<notin> FFVars t' \<or> z = v') \<and>
+       swap t z v = swap t' z v')"
+unfolding Lam_inject_swap apply(rule iffI)
+  subgoal apply clarsimp apply(rule exI[of _ v']) by auto
+  subgoal by (smt (verit, del_insts) Lam_inject_swap)    .
+
+lemma Lam_refresh': "v' \<notin> FFVars t \<or> v' = v \<Longrightarrow>
+   Lam v t = Lam v' (swap t v' v)"
+using Lam_inject_swap by auto
+
+lemma Lam_refresh:
+"xx \<notin> FFVars t \<or> xx = x \<Longrightarrow> Lam x t = Lam xx (swap t x xx)"
+by (metis Lam_inject_swap fun_upd_twist)
+
+(* *)
+
+lemma FFVars_usub[simp]: "FFVars (usub t y x) =
+ (if x \<in> FFVars t then FFVars t - {x} \<union> {y} else FFVars t)"
+apply(subst term.set_map) by auto
+
+lemma usub_simps_free[simp]: "\<And>y x. usub (Var z) (y::var) x = Var (sb z y x)"
+"\<And>y x t s. usub (App t s) (y::var) x = App (usub t y x) (usub s y x)"
+by (auto simp: sb_def)
+
+lemma usub_Lam[simp]:
+"v \<notin> {x,y} \<Longrightarrow> usub (Lam v t) (y::var) x = Lam v (usub t y x)"
+apply(subst term.map)
+  subgoal by auto
+  subgoal by (auto simp: imsupp_def supp_def)
+  subgoal by auto .
+
+lemmas usub_simps = usub_simps_free usub_Lam
+
+(* *)
+
+lemma rrename_usub[simp]:
+assumes \<sigma>: "bij \<sigma>" "|supp \<sigma>| <o |UNIV::var set|"
+shows "rrename \<sigma> (usub t u (x::var)) = usub (rrename \<sigma> t) (\<sigma> u) (\<sigma> x)"
+using assms
+apply(binder_induction t avoiding: "supp \<sigma>" u x rule: term.strong_induct)
+using assms by (auto simp: sb_def)
+
+lemma sw_sb:
+"sw (sb z u x) z1 z2 = sb (sw z z1 z2) (sw u z1 z2) (sw x z1 z2)"
+unfolding sb_def sw_def by auto
+
+
+lemma swap_usub:
+"swap (usub t (u::var) x) z1 z2 = usub (swap t z1 z2) (sw u z1 z2) (sw x z1 z2)"
+apply(binder_induction t avoiding: u x z1 z2 rule: term.strong_induct)
+  subgoal
+  apply(subst swap_simps) apply(subst usub_simps) by (auto simp: sb_def)
+  subgoal apply(subst swap_simps | subst usub_simps)+ by presburger
+  subgoal apply(subst swap_simps | subst usub_simps)+
+    subgoal by auto
+    subgoal apply(subst swap_simps | subst usub_simps)+
+      subgoal unfolding sw_def sb_def by auto
+      unfolding sw_sb by presburger . .
+
+lemma usub_refresh:
+assumes "xx \<notin> FFVars t \<or> xx = x"
+shows "usub t u x = usub (swap t x xx) u xx"
+proof-
+  note term_vvsubst_rrename[simp del]
+  show ?thesis using assms
+  apply(subst term_vvsubst_rrename[symmetric]) apply simp
+    subgoal by auto
+    subgoal apply(subst term.map_comp)
+      subgoal by auto
+      subgoal by auto
+      subgoal apply(rule term.map_cong0)
+      using term_pre.supp_comp_bound by auto . .
+qed
+
+lemma swap_commute:
+"{y,yy} \<inter> {x,xx} = {} \<Longrightarrow>
+ swap (swap t y yy) x xx = swap (swap t x xx) y yy"
+apply(subst term.rrename_comps)
+apply auto
+apply(subst term.rrename_comps)
+apply auto
+apply(rule rrename_cong)
+by (auto simp: term_pre.supp_comp_bound)
+
+
+(* *)
+
+term "swappingFvars swap FFVars"
+term "permutFvars (\<lambda>f t. rrename t f) FFVars"
+
+lemma swappingFvars_swap_FFVars: "swappingFvars swap FFVars"
+unfolding swappingFvars_def apply auto
+  apply (metis id_swapTwice rrename_o_swap term.rrename_ids) 
+  using sw_invol2 apply metis 
+  by (metis (no_types, lifting) image_iff sw_invol2)
+
+lemma nswapping_swap: "nswapping swap"
+unfolding nswapping_def apply auto
+apply (metis id_swapTwice rrename_o_swap term.rrename_ids)
+by (metis id_swapTwice2 rrename_o_swap)
+
+lemma permutFvars_rrename_FFVar: "permutFvars (\<lambda>t f. rrename f (t::trm)) FFVars"
+unfolding permutFvars_def apply auto
+  apply (simp add: finite_iff_le_card_var fsupp_def supp_def term.rrename_comps) 
+  apply (simp add: finite_iff_le_card_var fsupp_def supp_def)
+  apply (simp add: finite_iff_le_card_var fsupp_def image_in_bij_eq supp_def) .
+
+lemma permut_rrename: "permut (\<lambda>t f. rrename f (t::trm))"
+unfolding permut_def apply auto
+by (simp add: finite_iff_le_card_var fsupp_def supp_def term.rrename_comps)
+
+lemma toSwp_rrename: "toSwp (\<lambda>t f. rrename f t) = swap"
+by (meson toSwp_def)
+
+lemma fsupp_supp: "fsupp f \<longleftrightarrow> |supp f| <o |UNIV::var set|"
+unfolding fsupp_def supp_def using finite_iff_le_card_var by blast
+
+lemma toPerm_swap: "bij f \<Longrightarrow> |supp f| <o |UNIV::var set| \<Longrightarrow> toPerm swap t f = rrename f t"
+apply(subst toSwp_rrename[symmetric])
+by (simp add: fsupp_supp permut_rrename toPerm_toSwp)
+
+
+(* *)
+(* Substitution from a sequence (here, a list) *)
+
+(* "making" the substitution function that maps each xs_i to es_i; only 
+meaningful if xs is non-repetitive *)
+definition "mkSubst xs es \<equiv> \<lambda>x. if distinct xs \<and> x \<in> set xs then nth es (theN xs x) else Var x"
+
+lemma mkSubst_nth[simp]: "distinct xs \<Longrightarrow> i < length xs \<Longrightarrow> mkSubst xs es (nth xs i) = nth es i"
+unfolding mkSubst_def by auto
+
+lemma mkSubst_idle[simp]: "\<not> distinct xs \<or> \<not> x \<in> set xs \<Longrightarrow> mkSubst xs es x = Var x"
+unfolding mkSubst_def by auto
+
+lemma card_set_var: "|set xs| <o |UNIV::var set|"
+by (simp add: infinite_var) 
+
+lemma SSupp_mkSubst[simp,intro]: "|SSupp (mkSubst xs es)| <o |UNIV::var set|"
+proof-
+  have "SSupp (mkSubst xs es) \<subseteq> set xs"
+  unfolding SSupp_def by auto (metis mkSubst_idle)
+  thus ?thesis by (simp add: card_of_subset_bound card_set_var)
+qed
+
+lemma mkSubst_map_rrename: 
+assumes s: "bij (\<sigma>::var\<Rightarrow>var)" "|supp \<sigma>| <o |UNIV::var set|" 
+and l: "length es2 = length xs"
+shows "mkSubst (map \<sigma> xs) (map (rrename \<sigma>) es2) \<circ> \<sigma> = rrename \<sigma> \<circ> mkSubst xs es2"
+proof(rule ext)  
+  fix x
+  show "(mkSubst (map \<sigma> xs) (map (rrename \<sigma>) es2) \<circ> \<sigma>) x = (rrename \<sigma> \<circ> mkSubst xs es2) x"
+  proof(cases "distinct xs \<and> x \<in> set xs")
+    case False
+    hence F: "\<not> distinct (map \<sigma> xs) \<or> \<not> \<sigma> x \<in> set (map \<sigma> xs)"
+    using s by auto
+    thus ?thesis using F False
+    unfolding o_def apply(subst mkSubst_idle) 
+      subgoal by auto
+      subgoal using s by auto .
+  next
+    case True
+    then obtain i where i: "i < length xs" and Tr: "distinct xs" and Tri: "x = nth xs i" by (metis theN)
+    hence T: "distinct (map \<sigma> xs)" and Ti: "\<sigma> x = nth (map \<sigma> xs) i"
+    using s by auto
+    thus ?thesis using T Tr
+    unfolding o_def Ti apply(subst mkSubst_nth) 
+      subgoal by auto
+      subgoal using i unfolding Tri by auto 
+      subgoal using l i unfolding Tri by auto .
+  qed
+qed
+
+lemma mkSubst_map_rrename_inv: 
+assumes "bij (\<sigma>::var\<Rightarrow>var)" "|supp \<sigma>| <o |UNIV::var set|" "length es2 = length xs"
+shows "mkSubst (map \<sigma> xs) (map (rrename \<sigma>) es2) = rrename \<sigma> \<circ> mkSubst xs es2 o inv \<sigma>"
+unfolding mkSubst_map_rrename[OF assms, symmetric] using assms unfolding fun_eq_iff by auto
+
+lemma card_SSupp_itvsubst_mkSubst_rrename_inv: 
+"bij (\<sigma>::var\<Rightarrow>var) \<Longrightarrow> |supp \<sigma>| <o |UNIV::var set| \<Longrightarrow> 
+ length es = length xs \<Longrightarrow> 
+|SSupp (tvsubst (rrename \<sigma> \<circ> mkSubst xs es \<circ> inv \<sigma>) \<circ> (Var \<circ> \<sigma>))| <o |UNIV::var set|"
+by (metis SSupp_tvsubst_bound SSupp_mkSubst mkSubst_map_rrename_inv supp_SSupp_Var_le)
+
+lemma card_SSupp_mkSubst_rrename_inv: 
+"bij (\<sigma>::var\<Rightarrow>var) \<Longrightarrow> |supp \<sigma>| <o |UNIV::var set| \<Longrightarrow> 
+ length es = length xs \<Longrightarrow> 
+ |SSupp (rrename \<sigma> \<circ> mkSubst xs es \<circ> inv \<sigma>)| <o |UNIV::var set|"
+by (metis SSupp_mkSubst mkSubst_map_rrename_inv)
+
+lemma mkSubst_smap: "bij f \<Longrightarrow> distinct xs \<Longrightarrow> z \<in> set xs \<Longrightarrow> 
+ length es = length xs \<Longrightarrow> 
+ mkSubst (map f xs) es (f z) = mkSubst xs es z"
+by (metis bij_distinct_smap distinct_Ex1 length_map mkSubst_nth nth_map) 
+
+
+(* *)
+
+lemma Lam_eq_tvsubst: 
+assumes il: "Lam (x::var) e1 = Lam x' e1'"
+shows "tvsubst (Var (x:=e2)) e1 = tvsubst (Var (x':=e2)) e1'"
+proof-
+  obtain f where f: "bij f" "|supp f| <o |UNIV::var set|" "id_on (FFVars (Lam x e1)) f" 
+  and 0: "x' = f x" "e1' = rrename f e1" using il[unfolded Lam_inject] by auto
+  show ?thesis unfolding 0 apply(subst rrename_eq_tvsubst_Var')
+    subgoal by fact subgoal by fact
+    subgoal apply(subst tvsubst_comp)
+      subgoal by simp
+      subgoal using f(2) by auto
+      subgoal apply(rule tvsubst_cong)
+        subgoal by simp
+        subgoal by (simp add: SSupp_tvsubst_bound f(2))
+        subgoal apply simp 
+     subgoal using f(1) f(3) id_onD by fastforce . . . .
+qed
+
+
+
+
+(* RECURSOR PREPARATIONS: *)
+
+thm Lam_inject[no_vars]
+
+lemma Lam_inject_strong:
+assumes "Lam (x::var) e = Lam x' e'"
+shows "\<exists>f. bij f \<and> |supp f| <o |UNIV::var set| \<and>  
+   id_on (- {x,x'}) f \<and> id_on (FFVars (Lam x e)) f \<and>
+   f x = x' \<and> rrename f e = e'" 
+apply(rule exI[of _ "id(x := x', x' := x)"])
+using assms unfolding Lam_inject_swap apply safe
+unfolding id_on_def by auto (metis fun_upd_twist)
+
+
+lemma Lam_inject_strong':
+assumes il: "Lam (x::var) e = Lam x' e'" and z: "z \<notin> FFVars (Lam x e) \<union> FFVars (Lam x' e')"
+shows 
+"\<exists>f f'. 
+   bij f \<and> |supp f| <o |UNIV::var set| \<and> id_on (- {x,z}) f \<and> id_on (FFVars (Lam x e)) f \<and> f x = z \<and> 
+   bij f' \<and> |supp f'| <o |UNIV::var set| \<and> id_on (- {x',z}) f' \<and> id_on (FFVars (Lam x' e')) f' \<and> f' x' = z \<and> 
+   rrename f e = rrename f' e'"
+proof-
+  define f where "f = id(x := z, z := x)"
+  have f: "bij f \<and> |supp f| <o |UNIV::var set| \<and> id_on (- {x,z}) f \<and> id_on (FFVars (Lam x e)) f \<and> f x = z"
+  using z unfolding f_def id_on_def by auto
+  define f' where "f' = id(x' := z, z := x')"
+  have f': "bij f' \<and> |supp f'| <o |UNIV::var set| \<and> id_on (- {x',z}) f' \<and> id_on (FFVars (Lam x' e')) f' \<and> f' x' = z"
+  using z unfolding f'_def id_on_def by auto
+ 
+  obtain g where g: "bij g \<and> |supp g| <o |UNIV::var set| \<and> id_on (FFVars (Lam x e)) g \<and> g x = x'" and ge: "e' = rrename g e"
+  using il unfolding Lam_inject by auto
+
+  have ff': "rrename f e = rrename f' e'" 
+  unfolding f_def f'_def ge unfolding f_def f'_def using g apply(subst term.rrename_comps)
+    subgoal by auto  subgoal by auto subgoal by auto subgoal by auto
+    subgoal apply(rule rrename_cong) using g
+      subgoal by auto  subgoal by auto subgoal by auto 
+      subgoal using term_pre.supp_comp_bound by auto
+      subgoal using term_pre.supp_comp_bound z unfolding id_on_def by auto . .
+
+  show ?thesis
+  apply(rule exI[of _ f]) apply(rule exI[of _ f'])
+  using f f' ff' by auto
+qed
+
+lemma trm_rrename_induct[case_names Var App Lam]:
+assumes VVar: "\<And>x. P (Var (x::var))"
+and AApp: "\<And>e1 e2. P e1 \<Longrightarrow> P e2 \<Longrightarrow> P (App e1 e2)" 
+and LLam: "\<And>x e. (\<And>f. bij f \<Longrightarrow> |supp f| <o |UNIV::var set| \<Longrightarrow> P (rrename f e)) \<Longrightarrow> P (Lam x e)"
+shows "P t"
+proof-
+  have "\<forall>f. bij f \<and> |supp f| <o |UNIV::var set| \<longrightarrow> P (rrename f t)"
+  proof(induct)
+    case (Var x)
+    then show ?case using VVar by auto
+  next
+    case (App t1 t2)
+    then show ?case using AApp by auto
+  next
+    case (Lam x t)
+    then show ?case using LLam
+      by simp (metis bij_o term.rrename_comps term_pre.supp_comp_bound)
+  qed
+  thus ?thesis apply(elim allE[of _ id]) by auto
+qed
+
+(* RECURSOR *)
+
+locale LC_Rec = 
+fixes B :: "'b set"
+and VarB :: "var \<Rightarrow> 'b" 
+and AppB :: "'b \<Rightarrow> 'b \<Rightarrow> 'b"
+and LamB :: "var \<Rightarrow> 'b \<Rightarrow> 'b"
+and renB :: "(var \<Rightarrow> var) \<Rightarrow> 'b \<Rightarrow> 'b"
+and FVarsB :: "'b \<Rightarrow> var set"
+assumes 
+(* closedness: *)
+VarB_B[simp,intro]: "\<And>x. VarB x \<in> B"
+and 
+AppB_B[simp,intro]: "\<And>b1 b2. {b1,b2} \<subseteq> B \<Longrightarrow> AppB b1 b2 \<in> B"
+and 
+LamB_B[simp,intro]: "\<And>x b. b \<in>  B \<Longrightarrow> LamB x b \<in> B"
+and 
+renB_B[simp]: "\<And>\<sigma> b. bij \<sigma> \<Longrightarrow> |supp \<sigma>| <o |UNIV::var set| \<Longrightarrow> b \<in> B \<Longrightarrow> renB \<sigma> b \<in> B"
+and 
+(* proper axioms: *)
+renB_id[simp,intro]: "\<And>b. b \<in> B \<Longrightarrow> renB id b = b"
+and 
+renB_comp[simp,intro]: "\<And>b \<sigma> \<tau>. bij \<sigma> \<Longrightarrow> |supp \<sigma>| <o |UNIV::var set| \<Longrightarrow> 
+    bij \<tau> \<Longrightarrow> |supp \<tau>| <o |UNIV::var set| \<Longrightarrow> b \<in> B \<Longrightarrow> renB (\<tau> o \<sigma>) b = renB \<tau> (renB \<sigma> b)"
+and 
+renB_cong[simp]: "\<And>\<sigma> b. bij \<sigma> \<Longrightarrow> |supp \<sigma>| <o |UNIV::var set| \<Longrightarrow> 
+   (\<forall>x \<in> FVarsB b. \<sigma> x = x) \<Longrightarrow> 
+   renB \<sigma> b = b"
+(* and 
+NB: This is redundant:  
+renB_FVarsB[simp]: "\<And>\<sigma> x b. bij \<sigma> \<Longrightarrow> |supp \<sigma>| <o |UNIV::var set| \<Longrightarrow> 
+   x \<in> FVarsB (renB \<sigma> b) \<longleftrightarrow> inv \<sigma> x \<in> FVarsB b"
+*)
+and 
+(* *)
+renB_VarB[simp]: "\<And>\<sigma> x. bij \<sigma> \<Longrightarrow> |supp \<sigma>| <o |UNIV::var set| \<Longrightarrow> renB \<sigma> (VarB x) = VarB (\<sigma> x)"
+and 
+renB_AppB[simp]: "\<And>\<sigma> b1 b2. bij \<sigma> \<Longrightarrow> |supp \<sigma>| <o |UNIV::var set| \<Longrightarrow> {b1,b2} \<subseteq> B \<Longrightarrow> 
+   renB \<sigma> (AppB b1 b2) = AppB (renB \<sigma> b1) (renB \<sigma> b2)"
+and 
+renB_LamB[simp]: "\<And>\<sigma> x b. bij \<sigma> \<Longrightarrow> |supp \<sigma>| <o |UNIV::var set| \<Longrightarrow> b \<in> B \<Longrightarrow> 
+   renB \<sigma> (LamB x b) = LamB (\<sigma> x) (renB \<sigma> b)"
+(* *)
+and 
+FVarsB_VarB: "\<And>x. FVarsB (VarB x) \<subseteq> {x}"
+and 
+FVarsB_AppB: "\<And>b1 b2. {b1,b2} \<subseteq> B \<Longrightarrow> FVarsB (AppB b1 b2) \<subseteq> FVarsB b1 \<union> FVarsB b2"
+and 
+FVarsB_LamB: "\<And>x b. b \<in> B \<Longrightarrow> FVarsB (LamB x b) \<subseteq> FVarsB b - {x}"
+begin 
+
+lemma not_in_FVarsB_LamB: "b \<in> B \<Longrightarrow> x \<notin> FVarsB (LamB x b)"
+using FVarsB_LamB by auto
+
+lemma LamB_inject_strong_rev: 
+assumes bb': "{b,b'} \<subseteq> B" and 
+x': "x' = x \<or> x' \<notin> FVarsB b" and 
+f: "bij f" "|supp f| <o |UNIV::var set|" 
+"id_on (- {x, x'}) f" "f x = x'" and r: "renB f b = b'"
+shows "LamB x b = LamB x' b'"
+proof-
+  have id: "id_on (FVarsB (LamB x b)) f"
+  using f FVarsB_LamB bb' x' unfolding id_on_def by auto
+  have "LamB x b = renB f (LamB x b)"
+  apply(rule sym) apply(rule renB_cong) using f bb' FVarsB_LamB unfolding id_on_def 
+  using id unfolding id_on_def by auto
+  also have "\<dots> = LamB x' b'" apply(subst renB_LamB) using f r bb' by auto
+  finally show ?thesis .
+qed
+
+lemma LamB_inject_strong'_rev: 
+assumes bb': "{b,b'} \<subseteq> B"  
+and z: "z = x \<or> z \<notin> FVarsB b" "z = x' \<or> z \<notin> FVarsB b'"
+and f: "bij f" "|supp f| <o |UNIV::var set|" "id_on (- {x, z}) f" "f x = z" 
+and f': "bij f'" "|supp f'| <o |UNIV::var set|" "id_on (- {x', z}) f'" "f' x' = z" 
+and r: "renB f b = renB f' b'"
+shows "LamB x b = LamB x' b'" 
+proof-
+  define c where c: "c = renB f b"
+  have c': "c = renB f' b'" unfolding c r ..
+  have "LamB x b = LamB z c"  
+  apply(rule LamB_inject_strong_rev[of _ _ _ _ f]) 
+  using assms FVarsB_LamB id_on_def unfolding c by auto
+  also have "LamB z c = LamB x' b'"  
+  apply(rule sym, rule LamB_inject_strong_rev[of _ _ _ _ f']) 
+  using assms FVarsB_LamB id_on_def unfolding c by auto
+  finally show ?thesis .
+qed
+
+(* NB: 
+We obtain a more general recursor if we replace renB_cong with LamB_inject_strong_rev; 
+and an even more general one if we replace it with LamB_inject_strong'_rev. 
+*)
+
+definition morFromTrm where 
+"morFromTrm H \<equiv> 
+ (\<forall>e. H e \<in> B) \<and>  
+ (\<forall>x. H (Var x) = VarB x) \<and> 
+ (\<forall>e1 e2. H (App e1 e2) = AppB (H e1) (H e2)) \<and> 
+ (\<forall>x e. H (Lam x e) = LamB x (H e)) \<and> 
+ (\<forall>\<sigma> e. bij \<sigma> \<and> |supp \<sigma>| <o |UNIV::var set| \<longrightarrow> H (rrename \<sigma> e) = renB \<sigma> (H e)) \<and> 
+ (\<forall>e. FVarsB (H e) \<subseteq> FFVars e)"
+
+(* *)
+
+inductive R where 
+Var: "R (Var x) (VarB x)"
+|
+App: "R e1 b1 \<Longrightarrow> R e2 b2 \<Longrightarrow> R (App e1 e2) (AppB b1 b2)"
+|
+Lam: "R e b \<Longrightarrow> R (Lam x e) (LamB x b)"
+
+(* *)
+
+lemma R_Var_elim[simp]: "R (Var x) b \<longleftrightarrow> b = VarB x"
+apply safe
+  subgoal using R.cases by fastforce
+  subgoal by (auto intro: R.intros) .
+
+lemma R_App_elim: 
+assumes "R (App e1 e2) b"
+shows "\<exists>b1 b2. R e1 b1 \<and> R e2 b2 \<and> b = AppB b1 b2"
+by (metis App_inject R.simps assms term.distinct(1) term.distinct(4))
+
+lemma R_Lam_elim: 
+assumes "R (Lam x e) b"
+shows "\<exists>x' e' b'. R e' b' \<and> Lam x e = Lam x' e' \<and> b = LamB x' b'"
+using assms by (cases rule: R.cases) auto
+
+lemma R_total: 
+"\<exists>b. R e b"
+apply(induct e) by (auto intro: R.intros)
+
+lemma R_B: 
+"R e b \<Longrightarrow> b \<in> B"
+apply(induct rule: R.induct) by auto
+
+lemma R_main: 
+"(\<forall>b b'. R e b \<longrightarrow> R e b' \<longrightarrow> b = b') \<and> 
+ (\<forall>b. R e b \<longrightarrow> FVarsB b \<subseteq> FFVars e) \<and> 
+ (\<forall>b f. R e b \<and> bij f \<and> |supp f| <o |UNIV::var set|
+        \<longrightarrow> R (rrename f e) (renB f b))"
+proof(induct e rule: trm_rrename_induct)
+  case (Var x)
+  then show ?case using FVarsB_VarB by auto
+next
+  case (App e1 e2)
+  then show ?case apply safe 
+    subgoal by (metis R_App_elim)
+    subgoal by simp (smt (verit, del_insts) FVarsB_AppB R_App_elim 
+      R_B Un_iff bot.extremum insert_Diff insert_subset)
+    subgoal apply(drule R_App_elim) 
+      by (smt (verit, del_insts) R.simps R_B bot.extremum insert_subset renB_AppB 
+      rrename_simps(2)) .
+next
+  case (Lam x t)
+  note Lamm = Lam[rule_format]
+  note Lam1 = Lamm[THEN conjunct1, rule_format]
+  note Lam2 = Lamm[THEN conjunct2, THEN conjunct1, rule_format]
+  note Lam3 = Lamm[THEN conjunct2, THEN conjunct2, rule_format, OF _ _ conjI, OF _ _ _ conjI]
+  note Lam33 = Lam3[of id, simplified]
+
+  show ?case proof safe
+    fix b1 b2 assume RLam: "R (Lam x t) b1" "R (Lam x t) b2" 
+    then obtain x1' t1' b1' x2' t2' b2'
+    where 1: "R t1' b1'" "Lam x t = Lam x1' t1'" "b1 = LamB x1' b1'"
+    and   2: "R t2' b2'" "Lam x t = Lam x2' t2'" "b2 = LamB x2' b2'"
+    using R_Lam_elim by metis
+
+    have b12': "{b1',b2'} \<subseteq> B"
+    using 1(1,3) 2(1,3) R_B by auto
+
+    have "|{x,x1',x2'} \<union> FFVars t \<union> FFVars t1' \<union> FFVars t2'| <o |UNIV::var set|"
+    by (metis Un_insert_right singl_bound sup_bot_right term.set_bd_UNIV var_term_pre_class.Un_bound)
+    then obtain z where z: 
+    "z \<notin> {x,x1',x2'} \<union> FFVars t \<union> FFVars t1' \<union> FFVars t2'" 
+    by (meson exists_fresh)
+
+    obtain f1 f1' where 
+    f1: "bij f1" "|supp f1| <o |UNIV::var set|"
+       "id_on (- {x, z}) f1 \<and> id_on (FFVars (Lam x t)) f1" and 
+    f1': "bij f1'" "|supp f1'| <o |UNIV::var set|"
+       "id_on (- {x1', z}) f1' \<and> id_on (FFVars (Lam x1' t1')) f1'"
+    and z1: "f1 x = z" "f1' x1' = z"  
+    and f1f1': "rrename f1 t = rrename f1' t1'"   
+    using z Lam_inject_strong'[OF 1(2), of z] by auto
+
+    have if1': "bij (inv f1' o f1)" "|supp (inv f1' o f1)| <o |UNIV::var set|"
+    by (auto simp add: f1 f1' term_pre.supp_comp_bound)
+
+    have t1': "t1' = rrename (inv f1' o f1) t"  
+    using f1f1' by (metis (mono_tags, lifting) bij_imp_bij_inv f1 f1' 
+       inv_o_simp1 supp_inv_bound term.rrename_comps term.rrename_ids)
+
+    have fvb1': "FVarsB b1' \<subseteq> FFVars t1'"
+    using Lam2[OF if1', unfolded t1'[symmetric], OF 1(1)] .
+
+    obtain f2 f2' where 
+    f2: "bij f2" "|supp f2| <o |UNIV::var set|"
+      "id_on (- {x, z}) f2 \<and> id_on (FFVars (Lam x t)) f2" and 
+    f2': "bij f2'" "|supp f2'| <o |UNIV::var set|"
+      "id_on (- {x2', z}) f2' \<and> id_on (FFVars (Lam x2' t2')) f2'"
+    and z2: "f2 x = z" "f2' x2' = z"  
+    and f2f2': "rrename f2 t = rrename f2' t2'"   
+    using z Lam_inject_strong'[OF 2(2), of z] by auto
+
+    have if2': "bij (inv f2' o f2)" "|supp (inv f2' o f2)| <o |UNIV::var set|"
+    by (auto simp add: f2 f2' term_pre.supp_comp_bound)
+
+    have t2': "t2' = rrename (inv f2' o f2) t" 
+    using f2f2' by (metis (mono_tags, lifting) bij_imp_bij_inv f2 f2' 
+      inv_o_simp1 supp_inv_bound term.rrename_comps term.rrename_ids)
+
+    have fvb2': "FVarsB b2' \<subseteq> FFVars t2'"
+    using Lam2[OF if2', unfolded t2'[symmetric], OF 2(1)] .
+
+    define ff2' where "ff2' = f1 o (inv f2) o f2'"
+
+    have ff2': "bij ff2'" "|supp ff2'| <o |UNIV::var set|"
+       "id_on (- {x2', z}) ff2' \<and> id_on (FFVars (Lam x2' t2')) ff2'" 
+    unfolding ff2'_def using f1 f2 f2'  
+      subgoal by auto 
+      subgoal unfolding ff2'_def using f1 f2 f2' by (simp add: term_pre.supp_comp_bound)
+      subgoal unfolding ff2'_def using f1 f2 f2' unfolding id_on_def by simp (metis inv_simp1 z1(1) z2(1)) .
+
+    have zz2: "ff2' x2' = z"
+    by (metis comp_def f2 ff2'_def inv_simp1 z1(1) z2(1) z2(2))
+ 
+    have rew1: "rrename f1' (rrename (inv f1' \<circ> f1) t) = rrename f1 t" 
+    using f1f1' t1' by auto
+
+    have rew2: "rrename ff2' (rrename (inv f2' \<circ> f2) t) = rrename f1 t" 
+    by (smt (verit, del_insts) bij_betw_imp_inj_on bij_imp_bij_inv bij_o f1(1) f1(2) f2'(1) f2'(2) f2(1) f2(2) f2f2' ff2'_def o_inv_o_cancel supp_inv_bound term.rrename_comps term_pre.supp_comp_bound)
+ 
+    show "b1 = b2" unfolding 1(3) 2(3) 
+    apply(rule LamB_inject_strong'_rev[OF b12', of z _ _ f1' ff2'])
+      subgoal using z fvb1' by auto
+      subgoal using z fvb2' by auto
+      subgoal using f1' by auto  subgoal using f1' by auto
+      subgoal using f1' by auto  subgoal using z1 by auto
+      subgoal using ff2' by auto  subgoal using ff2' by auto
+      subgoal using ff2' by auto  subgoal using zz2 by auto 
+      subgoal apply(rule Lam1[OF f1(1,2)])  
+        subgoal using Lam3[OF if1' 1(1)[unfolded t1'] f1'(1,2), unfolded rew1] .
+        subgoal using Lam3[OF if2' 2(1)[unfolded t2'] ff2'(1,2), unfolded rew2] . . .
+  (* *)
+  next
+    fix b y 
+    assume R: "R (Lam x t) b" and yy: "y \<in> FVarsB b"
+    then obtain x' t' b'
+    where 0: "R t' b'" "Lam x t = Lam x' t'" "b = LamB x' b'" 
+    using R_Lam_elim by metis
+
+    have b': "b' \<in>  B"
+    using 0(1,3) R_B by auto
+
+    have y: "y \<noteq> x'" "y \<in> FVarsB b'" using b' yy unfolding 0 
+    using FVarsB_LamB[OF b'] by auto
+
+    have "|{x,x'} \<union> FFVars t \<union> FFVars t'| <o |UNIV::var set|"
+    by (metis Un_insert_right singl_bound sup_bot_right term.set_bd_UNIV var_term_pre_class.Un_bound)
+    then obtain z where z: 
+    "z \<notin> {x,x'} \<union> FFVars t \<union> FFVars t'" 
+    by (meson exists_fresh)
+
+    obtain f where 
+    f: "bij f" "|supp f| <o |UNIV::var set|"
+       "id_on (- {x, x'}) f \<and> id_on (FFVars (Lam x t)) f" 
+    and z: "f x = x'"   
+    and t': "t' = rrename f t" 
+    using  Lam_inject_strong[OF 0(2)] by auto
+    
+    have fvb't': "FVarsB b' \<subseteq> FFVars t'"
+    using Lam2[OF f(1,2), unfolded t'[symmetric], OF 0(1)] .
+    have yt': "y \<in> FFVars t'" using fvb't' y(2) by auto
+
+    show "y \<in> FFVars (Lam x t)" using yt' y unfolding 0(2) by auto
+  (* *)
+  next
+    fix b and f :: "var\<Rightarrow>var"
+
+    assume "R (Lam x t) b" and f: "bij f" "|supp f| <o |UNIV::var set|"
+
+   
+    then obtain x' t' b'
+    where 0: "R t' b'" "Lam x t = Lam x' t'" "b = LamB x' b'" 
+    using R_Lam_elim by metis
+
+
+    have b': "b' \<in>  B"
+    using 0(1,3) R_B by auto
+
+    have "|{x,x'} \<union> FFVars t \<union> FFVars t'| <o |UNIV::var set|"
+    by (metis Un_insert_right singl_bound sup_bot_right term.set_bd_UNIV var_term_pre_class.Un_bound)
+    then obtain z where z: 
+    "z \<notin> {x,x'} \<union> FFVars t \<union> FFVars t'" 
+    by (meson exists_fresh)
+
+    obtain g where 
+    g: "bij g" "|supp g| <o |UNIV::var set|"
+       "id_on (- {x, x'}) g \<and> id_on (FFVars (Lam x t)) g" 
+    and z: "g x = x'"   
+    and t': "t' = rrename g t" 
+    using Lam_inject_strong[OF 0(2)] by auto
+
+    have RR: "R (Lam (f x') (rrename f t')) (LamB (f x') (renB f b'))"
+    apply(rule R.Lam) unfolding t' apply(rule Lam3)
+      subgoal by fact  subgoal by fact
+      subgoal using 0(1) unfolding t' .
+      subgoal by fact subgoal by fact .
+
+    show "R (rrename f (Lam x t)) (renB f b)" 
+    unfolding 0 using RR apply(subst rrename_simps) 
+      subgoal using f by auto subgoal using f by auto
+      subgoal apply(subst renB_LamB)
+       using f b' by auto .  
+  qed
+qed
+
+lemmas R_functional = R_main[THEN conjunct1]
+lemmas R_FFVars = R_main[THEN conjunct2, THEN conjunct1]
+lemmas R_subst = R_main[THEN conjunct2, THEN conjunct2]
+
+definition H :: "trm \<Rightarrow> 'b" where "H t \<equiv> SOME d. R t d"
+
+lemma R_F: "R t (H t)"
+by (simp add: R_total H_def someI_ex)
+
+lemma ex_morFromTrm: "\<exists>H. morFromTrm H"
+apply(rule exI[of _ H]) unfolding morFromTrm_def apply(intro conjI)
+  subgoal using R_B R_F by auto
+  subgoal using R.Var R_F R_functional by blast
+  subgoal using R.App R_F R_functional by blast
+  subgoal using R.Lam R_F R_functional by blast
+  subgoal by (meson R_F R_functional R_subst)
+  subgoal by (simp add: R_F R_FFVars) .
+
+definition rec where "rec \<equiv> SOME H. morFromTrm H"
+
+lemma morFromTrm_rec: "morFromTrm rec"
+by (metis ex_morFromTrm rec_def someI_ex)
+
+lemma rec_B[simp,intro!]: "rec e \<in> B"
+using morFromTrm_rec unfolding morFromTrm_def by auto
+
+lemma rec_Var[simp]: "rec (Var x) = VarB x"
+using morFromTrm_rec unfolding morFromTrm_def by auto
+
+lemma rec_App[simp]: "rec (App e1 e2) = AppB (rec e1) (rec e2)"
+using morFromTrm_rec unfolding morFromTrm_def by auto
+
+lemma rec_Lam[simp]: "rec (Lam x e) = LamB x (rec e)"
+using morFromTrm_rec unfolding morFromTrm_def by auto
+
+lemma rec_rrename: "bij \<sigma> \<Longrightarrow> |supp \<sigma>| <o |UNIV::var set| \<Longrightarrow> 
+ rec (rrename \<sigma> e) = renB \<sigma> (rec e)"
+using morFromTrm_rec unfolding morFromTrm_def by auto
+
+lemma FVarsB_rec: "FVarsB (rec e) \<subseteq> FFVars e"
+using morFromTrm_rec unfolding morFromTrm_def by auto
+
+lemma rec_unique: 
+assumes "\<And>e. H e \<in> B" 
+"\<And>x. H (Var x) = VarB x" 
+"\<And>e1 e2. H (App e1 e2) = AppB (H e1) (H e2)"
+"\<And>x e. H (Lam x e) = LamB x (H e)"
+shows "H = rec"
+apply(rule ext) subgoal for e apply(induct e)
+using assms by auto .
+
+
+end (* context LC_Rec *)
+
+
+
+
+
+end
